ems/SimModSem.v
@@ -694,6 +694,7 @@ Section SIM.
     gstep. destruct st_src0, st_tgt0. econs; eauto. 
   Qed.
 
+
   Lemma sim_itree_flag_mon
         (sim_itree: forall (R_src R_tgt: Type)
                            (RR: st_local -> st_local -> R_src -> R_tgt -> Prop), bool -> bool -> world -> st_local * itree Es R_src -> st_local * itree Es R_tgt -> Prop)
